forwarding packets

interface_abstraction/Entity.thy
@@ -8,9 +8,17 @@ section{*Basic Definitions*}
       Network Boxes are neccessary for perating the networkg (e.g, switches, routers)
       'v is the name (e.g. ''Hans'', 192.168.0.1)*}
   datatype 'v entity = Host 'v | NetworkBox 'v
+
+  definition entity_name :: "'v entity \<Rightarrow> 'v" where
+    "entity_name e \<equiv> case e of Host h \<Rightarrow> h | NetworkBox h \<Rightarrow> h"
+
+  lemma "entity_name (Host X) = entity_name  (NetworkBox X)" by (simp add: entity_name_def)
   
   text{*A port, like a switche's port or a simple NIC*}
   datatype port = Port nat
+
+  text{*Example: port matching*}
+  value "(\<lambda> p. if p = Port 1 then True else False) (Port 1)"
   
   text{*We will move packets between interfaces.
     An interface is a certain port at an entity.*}
@@ -20,6 +28,5 @@ section{*Basic Definitions*}
   
   text{*Example: Port two in a three-port switch*}
   value "\<lparr> entity = NetworkBox ''threePortSwitch'', port = Port 2 \<rparr>"
-
 
 end
