interface_abstraction/Network.thy
@@ -23,6 +23,7 @@ section{*A network consisting of entities*}
     assumes fst_links: "fst ` links N \<subseteq> interfaces N"
     and     snd_links: "snd ` links N \<subseteq> interfaces N"
     and     finite_interfaces: "finite (interfaces N)"
+    and     names_disjunct: "{host. Host host \<in> entity ` interfaces N} \<inter> {box. NetworkBox box \<in> entity ` interfaces N} = {}"
     begin
       lemma finite_links: "finite (links N)"
       proof - 
@@ -32,6 +33,29 @@ section{*A network consisting of entities*}
           by (metis finite_cartesian_product rev_finite_subset)
       qed
 
+      lemma finite_entity_interfaces: "finite (entity ` interfaces N)" by(simp add: finite_interfaces)
+      lemma finite_entity_name_entity_interfaces: "finite (entity_name ` entity ` interfaces N)" by(simp add: finite_entity_interfaces)
+      
+      lemma names_disjunct_2: "\<forall>x\<in>interfaces N. \<forall>y\<in>interfaces N. entity_name (entity x) = entity_name (entity y) \<longrightarrow> entity x = entity y"
+        apply(clarify)
+        apply(case_tac x, rename_tac entity_x port_x, case_tac y, rename_tac entity_y port_y, clarsimp)
+        apply(case_tac entity_x, case_tac entity_y)
+        apply(simp add: entity_name_def)
+        apply(simp add: entity_name_def)
+        using names_disjunct apply force
+        apply(clarsimp)
+        apply(case_tac entity_y)
+        apply(simp add: entity_name_def)
+        using names_disjunct apply force
+        apply(simp add: entity_name_def)
+        done
+      lemma "card (entity ` interfaces N) = card (entity_name ` entity ` interfaces N)"
+        thm Set_Interval.BIJ
+        apply(subst Set_Interval.BIJ[OF finite_entity_interfaces finite_entity_name_entity_interfaces, symmetric])
+        apply(rule_tac x="entity_name" in exI)
+        apply(simp add: bij_betw_def inj_on_def)
+        apply(fact names_disjunct_2)
+        done
 
       text{*transmitting a packet. A packet is ready to be send at output port out. It is send to all ports that are connected. *}
       definition link_from :: "'v interface \<Rightarrow> ('v interface) set" where
@@ -43,23 +67,14 @@ section{*A network consisting of entities*}
         also have "{inI \<in> snd ` links N. (out, inI) \<in> links N} = {inI \<in> interfaces N. (out, inI) \<in> links N}" using snd_links by force
         finally show ?thesis using link_from_def by simp
       qed
-
-      definition add_iface :: "'v interface \<Rightarrow> 'v network" where
-        "add_iface i = \<lparr> interfaces = insert i (interfaces N), forwarding = forwarding N, links = links N \<rparr>"
-    
-      lemma add_wf: "wellformed_network (add_iface i)"
-        apply(unfold_locales)
-        apply(simp_all add: finite_interfaces add_iface_def)
-        using fst_links snd_links by auto
     end
 
     text{*the same link_from but conveniently executable*}
-    definition link_from :: "'v network \<Rightarrow> 'v interface \<Rightarrow> ('v interface) set" where
-      "link_from N out \<equiv> {inI \<in> interfaces N. (out, inI) \<in> links N}"
+    definition link_from_code :: "'v network \<Rightarrow> 'v interface \<Rightarrow> ('v interface) set" where
+      "link_from_code N out \<equiv> {inI \<in> interfaces N. (out, inI) \<in> links N}"
 
-    lemma "wellformed_network N \<Longrightarrow> wellformed_network.link_from N out = link_from N out"
-      by(simp add: wellformed_network.link_from_bounded link_from_def)
-
+    lemma "wellformed_network N \<Longrightarrow> wellformed_network.link_from N out = link_from_code N out"
+      by(simp add: wellformed_network.link_from_bounded link_from_code_def)
 
   text{*Example*}
     definition "example_network = \<lparr> interfaces = {\<lparr> entity = NetworkBox ''threePortSwitch'', port = Port 1 \<rparr>,
@@ -68,7 +83,11 @@ section{*A network consisting of entities*}
                            \<lparr> entity = Host ''Alice'', port = Port 1 \<rparr>,
                            \<lparr> entity = Host ''Bob'', port = Port 1 \<rparr>,
                            \<lparr> entity = Host ''Carl'', port = Port 1 \<rparr>},
-             forwarding = (\<lambda> e. \<lambda> p (srd,dst). {}),
+             forwarding = (\<lambda> e. 
+                if e = NetworkBox ''threePortSwitch'' then 
+                  (\<lambda> p (src,dst). if p = Port 1 then Port ` {2,3} else if p = Port 2 then Port ` {1,3} else if p = Port 3 then Port ` {1,2} else {})
+                else
+                  (\<lambda> p (src,dst). if e = Host src then {Port 1} else {})), (*Hosts send out their own packets and drop the rest*)
              links = {
               (\<lparr> entity = Host ''Alice'', port = Port 1 \<rparr>, \<lparr> entity = NetworkBox ''threePortSwitch'', port = Port 1 \<rparr>),
               (\<lparr> entity = NetworkBox ''threePortSwitch'', port = Port 1 \<rparr>, \<lparr> entity = Host ''Alice'', port = Port 1 \<rparr>),
@@ -85,9 +104,39 @@ section{*A network consisting of entities*}
 
     value[code] "example.link_from \<lparr> entity = NetworkBox ''threePortSwitch'', port = Port 3 \<rparr>"
 
-    lemma "link_from example_network \<lparr> entity = NetworkBox ''threePortSwitch'', port = Port 3 \<rparr> = {\<lparr>entity = Host ''Bob'', port = Port (Suc 0)\<rparr>, \<lparr>entity = Host ''Carl'', port = Port (Suc 0)\<rparr>}" by eval
+    lemma "link_from_code example_network \<lparr> entity = NetworkBox ''threePortSwitch'', port = Port 3 \<rparr> = {\<lparr>entity = Host ''Bob'', port = Port 1\<rparr>, \<lparr>entity = Host ''Carl'', port = Port 1\<rparr>}" by eval
 
-    value[code] "example.add_iface \<lparr> entity = NetworkBox ''threePortSwitch'', port = Port 4 \<rparr>"
+
+    subsection{*A packet traverses a hop*}
+      text{*A packet leaving an interface (outgoing) and traversing a link and arriving at an incoming interface. *}
+      definition succ :: "'v network \<Rightarrow> 'v interface \<Rightarrow> ('v interface) set" where
+        "succ N out_iface \<equiv> {in_iface. (out_iface, in_iface) \<in> links N}"
+        
+      definition succ_code :: "'v network \<Rightarrow> 'v interface \<Rightarrow> ('v interface) set" where
+        "succ_code N out_iface \<equiv> {in_iface \<in> interfaces N. (out_iface, in_iface) \<in> links N}"
+      lemma "wellformed_network N \<Longrightarrow> succ N = succ_code N"
+        apply(simp add: fun_eq_iff succ_def succ_code_def)
+        apply(drule wellformed_network.snd_links)
+        by force
+
+      lemma "succ_code example_network \<lparr> entity = NetworkBox ''threePortSwitch'', port = Port 3 \<rparr> = {\<lparr>entity = Host ''Bob'', port = Port 1\<rparr>, \<lparr>entity = Host ''Carl'', port = Port 1\<rparr>}" by eval
+
+      type_synonym 'v hdr="('v \<times> 'v)" -- "packet header: (src address, dst address)"
+      text{*A packet in network N with header hdr traverses hop hop. The output is the set of input interface at the nex hops*}
+      definition traverse :: "'v network \<Rightarrow> 'v hdr \<Rightarrow> 'v interface \<Rightarrow> ('v interface) set" where
+        "traverse N hdr hop \<equiv> UNION (((forwarding N) (entity hop)) (port hop) hdr) (\<lambda>p. succ N \<lparr>entity = entity hop, port = p\<rparr>)"
+
+      text{*Example: alice sends out packet, it arrives at switch*}
+      lemma "let N = example_network in let hdr = (''Alice'', ''Bob'') in let hop = \<lparr> entity = Host ''Alice'', port = Port 1 \<rparr> in 
+        (UNION (((forwarding N) (entity hop)) (port hop) hdr) (\<lambda>p. succ_code N \<lparr>entity = entity hop, port = p\<rparr>))  = {\<lparr>entity = NetworkBox ''threePortSwitch'', port = Port 1\<rparr>}" by eval
+      text{*Example cont.: Switch forwards packet to Bob and Carl*}
+      lemma "let N = example_network in let hdr = (''Alice'', ''Bob'') in let hop = \<lparr>entity = NetworkBox ''threePortSwitch'', port = Port 1\<rparr> in 
+        (UNION (((forwarding N) (entity hop)) (port hop) hdr) (\<lambda>p. succ_code N \<lparr>entity = entity hop, port = p\<rparr>)) = {\<lparr>entity = Host ''Carl'', port = Port 1\<rparr>, \<lparr>entity = Host ''Bob'', port = Port 1\<rparr>}" by eval
+      text{*Example cont.: Carl accepts packet (or drops it, he does not forward it)*}
+      lemma "let N = example_network in let hdr = (''Alice'', ''Bob'') in let hop = \<lparr>entity = Host ''Bob'', port = Port 1\<rparr> in 
+        (UNION (((forwarding N) (entity hop)) (port hop) hdr) (\<lambda>p. succ_code N \<lparr>entity = entity hop, port = p\<rparr>)) = {}" by eval
+
+
 
 section{*TEST of UNIO*}
   lemma "UNION {1::nat,2,3} (\<lambda>n. {n+1}) = {2,3,4}" by eval
